**放缩法**是通过舍去或添加一些项来构造[不等式的一种方法](https://zh.wikipedia.org/wiki/不等式 "wikilink")。

## 例子

1.  求证\(\sqrt{\log_2 3}+\sqrt{\log_3 2}<\sqrt{2}+1\)
    \[\sqrt{\log_2 3}+\sqrt{\log_3 2}<\sqrt{\log_2 4}+\sqrt{\log_3 3}=\sqrt{2}+1\]
2.  已知a,b,c,d为[正数](https://zh.wikipedia.org/wiki/正数 "wikilink")，求证\(1<\frac{a}{a+b+d}+\frac{b}{a+b+c}+\frac{c}{b+c+d}+\frac{d}{a+c+d}<2\)
    \[\frac{a}{a+b+d}+\frac{b}{a+b+c}+\frac{c}{b+c+d}+\frac{d}{a+c+d}>\frac{a}{a+b+c+d}+\frac{b}{a+b+c+d}+\frac{c}{a+b+c+d}+\frac{d}{a+b+c+d}=1\]
    \[\frac{a}{a+b+d}+\frac{b}{a+b+c}+\frac{c}{b+c+d}+\frac{d}{a+c+d}<\frac{a}{a+b}+\frac{b}{a+b}+\frac{c}{c+d}+\frac{d}{c+d}=2\]
3.  求证\(\sum_{k=1}^n \frac{1}{k^2}<2-\frac{1}{n}\)
    \[\sum_{k=1}^n \frac{1}{k^2}<1+\sum_{k=2}^n \frac{1}{k(k-1)}=1+\sum_{k=2}^n \frac{1}{k-1}-\frac{1}{k}=2-\frac{1}{n}\]

4.  设\(n \in N^+\)，求证\(\frac{n(n+1)}{2}< \sum_{k=1}^n \sqrt{k(k+1)} < \frac{(n+1)^2}{2}\)
    \[k=\sqrt{k^2}<\sqrt{k(k+1)}<\sqrt{k^2+k+\frac{1}{4}}=k+\frac{1}{2}\]
    \[\frac{n(n+1)}{2}=\sum_{k=1}^n k < \sum_{k=1}^n \sqrt{k(k+1)} < \sum_{k=1}^n (k+\frac{1}{2}) =\frac{n^2+2n}{2}<\frac{(n+1)^2}{2}\]

5.  设a,b,c为[直角三角形](../Page/直角三角形.md "wikilink")的三边,c为[斜边](https://zh.wikipedia.org/wiki/斜边 "wikilink")，求证：\(a^n+b^n<c^n(n>2)\)
    \[a^n+b^n=a^2 a^{n-2}+b^2 b^{n-2}<a^2 c^{n-2}+b^2 c^{n-2}=c^n(n>2)\]


## 备注

## 参考资料

[分类:不等式](https://zh.wikipedia.org/wiki/分类:不等式 "wikilink")