**权方和不等式**是一种分式不等式。

\(a_i,b_i>0\)

\(\begin{cases}
\displaystyle \sum_{i=1}^n \frac{a_i^{m+1}}{b_i^m} \ge \frac{(\displaystyle \sum_{i=1}^n a_i)^{m+1}}{(\displaystyle \sum_{i=1}^n b_i)^m},m<-1,m>0\\
\displaystyle \sum_{i=1}^n \frac{a_i^{m+1}}{b_i^m} \le \frac{(\displaystyle \sum_{i=1}^n a_i)^{m+1}}{(\displaystyle \sum_{i=1}^n b_i)^m},-1<m<0
\end{cases}\)\[1\]

取等条件：\(\frac{a_1}{b_1}=\frac{a_2}{b_2}=...=\frac{a_n}{b_n}\)

## 证明

利用[伯努利不等式](../Page/伯努利不等式.md "wikilink")：\[2\]

\(s=\frac{1}{a_1+a_2+...+a_n},t=\frac{1}{b_1+b_2+...+b_n}\)

m\<-1 或 m\>0时

\[\sum_{i=1}^n \frac{(sa_i)^{m+1}}{(tb_i)^m}=\sum_{i=1}^n tb_i(\frac{sa_i}{tb_i})^{m+1} \ge \sum_{i=1}^n tb_i[1+(m+1)(\frac{sa_i}{tb_i}-1)]\]

\[=\sum_{i=1}^n tb_i[(m+1)\frac{sa_i}{tb_i}-m]=\sum_{i=1}^n (m+1)sa_i-mtb_i=m+1-m=1\]

\[\sum_{i=1}^n \frac{a_i^{m+1}}{b_i^m} \ge \frac{t^m}{s^{m+1}}=\frac{(\displaystyle \sum_{i=1}^n a_i)^{m+1}}{(\displaystyle \sum_{i=1}^n b_i)^m}\]

\-1\<m\<0时

\[\sum_{i=1}^n \frac{(sa_i)^{m+1}}{(tb_i)^m}=\sum_{i=1}^n tb_i(\frac{sa_i}{tb_i})^m \le \sum_{i=1}^n tb_i[1+(m+1)(\frac{sa_i}{tb_i}-1)]\]

\[=\sum_{i=1}^n tb_i[(m+1)\frac{sa_i}{tb_i}-m]=\sum_{i=1}^n (m+1)sa_i-mtb_i=m+1-m=1\]

\(\sum_{i=1}^n \frac{a_i^{m+1}}{b_i^m} \le \frac{t^m}{s^{m+1}}=\frac{(\displaystyle \sum_{i=1}^n a_i)^{m+1}}{(\displaystyle \sum_{i=1}^n b_i)^m}\)

## 参见

  - [赫尔德不等式](../Page/赫尔德不等式.md "wikilink")

## 参考资料

[分类:代数不等式](https://zh.wikipedia.org/wiki/分类:代数不等式 "wikilink")

1.

2.